impl_putative_pn_offset

src/QUIC.Parse.fst
@@ -969,4 +969,59 @@ let write_header
 =
   admit ()
 
+let impl_putative_pn_offset
+  cid_len b len
+=
+  let sl = LowParse.Slice.make_slice b len in
+  let h0 = HST.get () in
+  if not (1ul `U32.lte` cid_len && cid_len `U32.lte` 4ul)
+  then 0ul
+  else
+    let _ = LL.valid_facts parse_u8 h0 sl 0ul in
+    let pos1 = LJ.validate_u8 () sl 0ul in
+    if pos1 `U32.gt` LL.validator_max_length
+    then 0ul
+    else
+      let _ =
+        parser_kind_prop_equiv parse_u8_kind parse_u8;
+        assert (pos1 == 1ul)
+      in
+      let hd = LJ.read_u8 sl 0ul in
+      if uint8.get_bitfield hd 7 8 = 0uy
+      then
+        let _ = LL.valid_facts (parse_bounded_integer (U32.v cid_len)) h0 sl pos1 in
+        let pos2 = LI.validate_bounded_integer' cid_len sl pos1 in
+        if pos2 `U32.gt` LL.validator_max_length
+        then 0ul
+        else pos2
+      else
+        let packet_type = uint8.get_bitfield hd 4 6 in
+        if packet_type = 3uy
+        then 0ul
+        else
+          let _ = LL.valid_facts parse_common_long h0 sl pos1 in
+          let pos2 = validate_common_long sl pos1 in
+          if pos2 `U32.gt` LL.validator_max_length
+          then 0ul
+          else
+            let pos3 =
+              if packet_type = 0uy
+              then
+                let _ = LL.valid_facts (parse_bounded_vlgenbytes 0 token_max_len (parse_bounded_varint 0 token_max_len)) h0 sl pos2 in
+                let pos3 = LB.validate_bounded_vlgenbytes 0 0ul token_max_len (U32.uint_to_t token_max_len) (validate_bounded_varint 0ul (U32.uint_to_t token_max_len)) (read_bounded_varint 0 token_max_len) sl pos2 in
+                if pos3 `U32.gt` LL.validator_max_length
+                then 0ul
+                else pos3
+              else
+                pos2
+            in
+            if pos3 = 0ul
+            then 0ul
+            else
+              let _ = LL.valid_facts parse_varint h0 sl pos3 in
+              let pos4 = validate_varint sl pos3 in
+              if pos4 `U32.gt` LL.validator_max_length
+              then 0ul
+              else pos4
+
 #pop-options
